

1 2.6

the notation used is $\langle v|w\rangle = (|v\rangle, |w\rangle)$

$$(\sum_i \lambda_i |w_i\rangle, |v\rangle) = (\sum_i \lambda_i |w_i\rangle)^\dagger |v\rangle = \sum_i \lambda_i^* \langle w_i|v\rangle = \sum_i \lambda_i^* (|w_i\rangle, |v\rangle)$$

2 2.7

–if $\langle w|v\rangle = 0$, then $|w\rangle$ and $|v\rangle$ are orthogonal

$$(1 \ 1) \begin{pmatrix} 1 \\ -1 \end{pmatrix} = 1 - 1 = 0$$

hence they are orthogonal!

–Normalized form of $\begin{pmatrix} a \\ b \end{pmatrix}$ is $\frac{1}{\sqrt{a^2 + b^2}} \begin{pmatrix} a \\ b \end{pmatrix}$ so, normalised form of the give matrices are :

$$|w\rangle = \frac{1}{\sqrt{2}} \begin{pmatrix} 1 \\ 1 \end{pmatrix}$$
$$|v\rangle = \frac{1}{\sqrt{2}} \begin{pmatrix} 1 \\ -1 \end{pmatrix}$$

3 2.9

If $|i\rangle$ are orthonormal basis that spans the vector space V . so, they will obey completeness relation. $\sum_i |i\rangle \langle i| = I$
also, any operator $A: V \rightarrow W$ such that $|v_i\rangle$ and $|w_i\rangle$ are orthonormal basis for the vector spaces V and W respectively. so we can write A as: $A = IAI$

$$A = \sum_i |v_i\rangle \langle v_i| A \sum_j |w_j\rangle \langle w_j|$$

$$A = \sum_{i,j} \langle v_i| A |w_j\rangle |v_i\rangle \langle w_j|$$

so, if the basis are $|0\rangle$ and $|1\rangle$ then pauli matrices can be represented as the outer product as follows:

$$X = \langle 0| X |0\rangle |0\rangle \langle 0| + \langle 1| X |0\rangle |1\rangle \langle 0| + \langle 0| X |1\rangle |0\rangle \langle 1| + \langle 1| X |1\rangle |1\rangle \langle 1|$$

$$X = |0\rangle \langle 1| + |1\rangle \langle 0|$$

similarly for Y:

$$Y|0\rangle = i|1\rangle \quad Y|1\rangle = -i|0\rangle$$

$$Y = \langle 0| Y |0\rangle |0\rangle \langle 0| + \langle 1| Y |0\rangle |1\rangle \langle 0| + \langle 0| Y |1\rangle |0\rangle \langle 1| + \langle 1| Y |1\rangle |1\rangle \langle 1|$$

$$Y = -i|0\rangle \langle 1| + i|1\rangle \langle 0|$$

similarly for Z: $Z|0\rangle = |0\rangle \quad Z|1\rangle = -|1\rangle$

$$Z = \langle 0| Z |0\rangle |0\rangle \langle 0| + \langle 1| Z |0\rangle |1\rangle \langle 0| + \langle 0| Z |1\rangle |0\rangle \langle 1| + \langle 1| Z |1\rangle |1\rangle \langle 1|$$

$$Z = |0\rangle \langle 0| - |1\rangle \langle 1|$$

4 2.10

given operator $A = (|v_j\rangle \langle v_k|)$

and since $|v_i\rangle$ forms the orthonormal basis for vector space V then, $\sum_i |v_i\rangle \langle v_i| = I$

A with respect to basis $|v_i\rangle$ can be written as :

$$A = \sum_i |v_i\rangle \langle v_i| (|v_j\rangle \langle v_k|) \sum_l |v_l\rangle \langle v_l|$$

$$A = \sum_{i,l} (\langle v_i | v_j \rangle) (\langle v_k | v_l \rangle) (|v_i\rangle \langle v_l|)$$

since, the basis in that spans vector space V are orthogonal, hence, $A = \sum_{i,l} \delta_{ij} \delta_{kl} |v_i\rangle \langle v_l|$

5 2.12

$$A = \begin{pmatrix} 1 & 0 \\ 1 & 1 \end{pmatrix} \text{ using } \det|A - \lambda I| = 0$$

$$\begin{vmatrix} 1 - \lambda & 0 \\ 1 & 1 - \lambda \end{vmatrix} = 0$$

$$(1 - \lambda)^2 = 0$$

$\lambda = 1, 1$ the eigenvalues are coming out to be degenerate. one of the eigenvector can be : $\begin{pmatrix} 0 \\ 1 \end{pmatrix}$ but there no other "eigenvector" for the given matrix A which is orthogonal to $\begin{pmatrix} 0 \\ 1 \end{pmatrix}$! so, this matrix is not diagonalizable.

6 2.13

$$(\langle v |)^{\dagger} = |v\rangle$$

$$(|w\rangle)^{\dagger} = \langle w|$$

$$(|w\rangle \langle v|)^{\dagger} = \langle v|^{\dagger} |w\rangle^{\dagger} = |v\rangle \langle w|$$

7 (2.15)

$A = \sum_i a_i |i\rangle \langle i|$ here $|i\rangle$ is the eigenvalues and a_i is the corresponding eigenvalues.

$$A^{\dagger} = \sum_i (a_i)^* |i\rangle \langle i|$$

$$(A^\dagger)^\dagger = \sum_i (a_i) |i\rangle \langle i|$$

$$(A^\dagger)^\dagger = A$$

8 2.16

projector operator $P = \sum_i |i\rangle \langle i|$ and each vector $|i\rangle$ is orthogonal to each other.

$$P^2 = P.P = \sum_i |i\rangle \langle i| \sum_j |j\rangle \langle j|$$

$$= \sum_{i,j} |i\rangle \langle i|j\rangle \langle j|$$

$$= \sum_{i,j} |i\rangle \langle j| \delta_{ij}$$

$$= \sum_i |i\rangle \langle i| = P$$

9 2.17

Any normal matrix follows the property $A^\dagger A = AA^\dagger$

$$A^\dagger A = AA^\dagger$$

$$A^{-1} A^\dagger A = A^{-1} A A^\dagger$$

$$A^{-1} A^\dagger A = A^\dagger \dots \dots \dots (1)$$

for A to be hermetian it follows from eq (1) that:

$$A^{-1} A^\dagger = I \implies A^\dagger = A$$

if $A = \sum_i a_i |i\rangle \langle i|$, where $|i\rangle$ are the eigenvectors of the A and a_i are the eigenvalues then, $A^\dagger = A \implies \sum_i a_i^* |i\rangle \langle i| = \sum_i a_i |i\rangle \langle i| \implies a_i^* = a_i$, and this condition is only possible if a is real !

10 2.18

if U is the unitary operator, $|v\rangle$ is the normalised eigenvector and a is its eigenvalue then,

$$U|v\rangle = a|v\rangle$$

$$\langle v|U^\dagger = a^*\langle v|$$

$$\langle v|U^\dagger U|v\rangle = a^*a\langle v|v\rangle$$

$$\implies 1 = a^*a \dots \dots \dots (1) \text{ since, } U^\dagger U = I$$

$$\text{so the modulus } |a| = |\sqrt{aa^*}| = 1$$

since, any complex number can be written as $re^{i\theta}$ following equation (1), we get :

$$|r^2 e^{i\theta} e^{-i\theta}| = |r^2| = 1 \implies |r| = 1$$

So, eigenvalues of U is $a = e^{i\theta}$, where θ is real